\chapter{The software renderer}

\newcommand{\dy}{\Delta y}
\newcommand{\dx}{\Delta x}

\enlargethispage{\baselineskip}

\section{Triangle rendering}

\begin{tikzpicture}
  \node (A) at (5,5) {$A$};
  \node (B) at (1,2) {$B$};
  \node (C) at (6,0) {$C$};
  \node (M) at (3,3.5) {};
  \node (N) at (5.3,3.5) {};
  \node (P) at (4.15,3.5) {};
  \draw (A) -- (B) node[pos=0.5,left]{$M$};
  \draw (A) -- (C) node[pos=0.28,right]{$N$};
  \draw (B) -- (C);
  \draw[dashed] (M) -- (N) node[pos=0.5]{$\bullet$} node[pos=0.5,above]{$P$};
  \node (YA) at (0,5) {};
  \node (YM) at (0,3.5) {};
  \node (XM) at (3,-1) {};
  \node (XP) at (4.15,-1) {};
  \draw[dotted] (YA) -- (A);
  \draw[dotted] (YM) -- (M);
  \draw[<->] (YA) -- (YM) node[pos=0.5,left]{$\dy$};
  \draw[dotted] (XM) -- (M);
  \draw[dotted] (XP) -- (P);
  \draw[<->] (XM) -- (XP) node[pos=0.5,above]{$\dx$};
\end{tikzpicture}

\begin{displaymath}
  \begin{array}{c}
    \begin{array}{c@{\quad\quad\quad}c}
      \left\{
        \begin{aligned}
          x_M & = x_A + \dy \times \frac{x_B - x_A}{y_B - y_A} \\
          v_M & = v_A + \dy \times \frac{v_B - v_A}{y_B - y_A} 
        \end{aligned}
      \right.
      &
      \left\{
        \begin{aligned}
          x_N & = x_A + \dy \times \frac{x_C - x_A}{y_C - y_A} \\
          v_N & = v_A + \dy \times \frac{v_C - v_A}{y_C - y_A} \\
        \end{aligned}
      \right.
    \end{array}
    \\
    \\
    v_P = v_M + \dx \times \frac{v_N - v_M}{x_N - x_M}
  \end{array}
\end{displaymath}

\begin{align*}
v_N - v_M & = \dy \times \left(\frac{v_C - v_A}{y_C - y_A} - \frac{v_B - v_A}{y_B - y_A}\right) \\
& = \dy \times \frac{(v_C - v_A)(y_B - y_A) - (v_B - v_A)(y_C - y_A)}{(y_B - y_A)(y_C - y_A)}
\\
x_N - x_M & = \dy \times \frac{(x_C - x_A)(y_B - y_A) - (x_B - x_A)(y_C - y_A)}{(y_B - y_A)(y_C - y_A)}
\end{align*}

\begin{align*}
\frac{v_N - v_M}{x_N - x_M} & = \frac{(v_C - v_A)(y_B - y_A) - (v_B - v_A)(y_C - y_A)}{(x_C - x_A)(y_B - y_A) - (x_B - x_A)(y_C - y_A)}
\end{align*}

Note that
\begin{align*}
(x_C - x_A)(y_B - y_A) - (x_B - x_A)(y_C - y_A) & =
\begin{array}{|cc|} 
  x_C - x_A & x_B - x_A \\
  y_C - y_A & y_B - y_A
\end{array}
\\
& = \det(AC, AB) \\
& = \|AC\| \|AB\| \sin(AC,AB) \\
& = - \|AB\| \|AC\| \sin(AB,AC) \\
& = - \det(AB, AC)
\end{align*}

The triangle is trivial iff this value is null. 

The sign of this value depends on the orientation of the triangle.

Thus, one might prefer one of the following expressions:
\begin{align*}
\frac{v_N - v_M}{x_N - x_M} 
& = \frac{(v_C - v_A)(y_B - y_A) - (v_B - v_A)(y_C - y_A)}{(x_C - x_A)(y_B - y_A) - (x_B - x_A)(y_C - y_A)} \\
& = \frac{(v_C - v_A)(y_B - y_A) - (v_B - v_A)(y_C - y_A)}{\det(AC,AB)} \\
& = \frac{(v_B - v_A)(y_C - y_A) - (v_C - v_A)(y_B - y_A)}{(x_B - x_A)(y_C - y_A) - (x_C - x_A)(y_B - y_A)} \\
& = \frac{(v_B - v_A)(y_C - y_A) - (v_C - v_A)(y_B - y_A)}{\det(AB,AC)}
\end{align*}

\section{Quadrilateral rendering}

\begin{tikzpicture}
  \node (A) at (5,5) {$A$};
  \node (B) at (1,2) {$B$};
  \node (C) at (10,0) {$C$};
  \node (D) at (9,5) {$D$};
  \node (M) at (3,3.5) {};
  \node (N) at (9.3,3.5) {};
  \node (P) at (6.15,3.5) {};
  \draw (A) -- (B) node[pos=0.5,left]{$M$};
  \draw (D) -- (C) node[pos=0.28,right]{$N$};
  \draw (B) -- (C);
  \draw (A) -- (D);
  \draw[dashed] (M) -- (N) node[pos=0.5]{$\bullet$} node[pos=0.5,above]{$P$};
  \node (YA) at (0,5) {};
  \node (YM) at (0,3.5) {};
  \node (XM) at (3,-1) {};
  \node (XP) at (6.15,-1) {};
  \draw[dotted] (YA) -- (A);
  \draw[dotted] (YM) -- (M);
  \draw[<->] (YA) -- (YM) node[pos=0.5,left]{$\dy$};
  \draw[dotted] (XM) -- (M);
  \draw[dotted] (XP) -- (P);
  \draw[<->] (XM) -- (XP) node[pos=0.5,above]{$\dx$};
\end{tikzpicture}

\begin{displaymath}
  \begin{array}{c}
    \begin{array}{c@{\quad\quad\quad}c}
      \left\{
        \begin{aligned}
          x_M & = x_A + \dy \times \frac{x_B - x_A}{y_B - y_A} \\
          v_M & = v_A + \dy \times \frac{v_B - v_A}{y_B - y_A} 
        \end{aligned}
      \right.
      &
      \left\{
        \begin{aligned}
          x_N & = x_D + \dy \times \frac{x_C - x_D}{y_C - y_D} \\
          v_N & = v_D + \dy \times \frac{v_C - v_D}{y_C - y_D} \\
        \end{aligned}
      \right.
    \end{array}
    \\
    \\
    v_P = v_M + \dx \times \frac{v_N - v_M}{x_N - x_M}
  \end{array}
\end{displaymath}

\begin{align*}
v_N - v_M & = v_D - v_A + \dy \times \left(\frac{v_C - v_D}{y_C - y_D} - \frac{v_B - v_A}{y_B - y_A}\right) \\
& = v_D - v_A + \dy \times \frac{(v_C - v_D)(y_B - y_A) - (v_B - v_A)(y_C - y_D)}{(y_B - y_A)(y_C - y_D)}
\\
x_N - x_M & = x_D - x_A + \dy \times \frac{(x_C - x_D)(y_B - y_A) - (x_B - x_A)(y_C - y_D)}{(y_B - y_A)(y_C - y_D)}
\end{align*}

\begin{align*}
\frac{v_N - v_M}{x_N - x_M} & = ? 
\end{align*}
